ValidReferences.v
@@ -1,6 +1,5 @@
 From Elo Require Import Core.
 
-From Elo Require Import Preservation.
 From Elo Require Import WellTypedTerm.
 
 (* ------------------------------------------------------------------------- *)
@@ -19,20 +18,38 @@ Inductive valid_references (m : mem) : tm -> Prop :=
                               valid_references m t2 ->
                               valid_references m <{call t1 t2}> 
 
-  | vr_refR  : forall T ad,   ad < #m                       ->
-                              empty |-- m[ad].t is `Safe T` ->
-                              m[ad].T = `r&T`               ->
+  | vr_refR  : forall ad t T, ad < #m                 ->
+                              m[ad].t = Some t        ->
+                              m[ad].T = `r&T`         ->
+                              empty |-- t is `Safe T` ->
                               valid_references m <{&ad : r&T}>
 
-  | vr_refX  : forall T ad,   ad < #m                ->
-                              empty |-- m[ad].t is T ->
-                              m[ad].T = `x&T`        ->
+  | vr_refX  : forall ad t T, ad < #m          ->
+                              m[ad].t = Some t ->
+                              m[ad].T = `x&T`  ->
+                              empty |-- t is T ->
                               valid_references m <{&ad : x&T}>
 
-  | vr_refW  : forall T ad,   ad < #m                ->
-                              empty |-- m[ad].t is T ->
-                              m[ad].T = `w&T`        ->
+  | vr_refW  : forall ad t T, ad < #m          ->
+                              m[ad].t = Some t ->
+                              m[ad].T = `w&T`  ->
+                              empty |-- t is T ->
                               valid_references m <{&ad : w&T}>
+
+  | vr_initR : forall ad t T, ad < #m              ->
+                              m[ad].T = `r&T`      ->
+                              valid_references m t ->
+                              valid_references m <{init ad t : `r&T`}> 
+
+  | vr_initX : forall ad t T, ad < #m              ->
+                              m[ad].T = `x&T`      ->
+                              valid_references m t ->
+                              valid_references m <{init ad t : `x&T`}> 
+
+  | vr_initW : forall ad t T, ad < #m              ->
+                              m[ad].T = `w&T`      ->
+                              valid_references m t ->
+                              valid_references m <{init ad t : `w&T`}> 
 
   | vr_new   : forall T t,    valid_references m t ->
                               valid_references m <{new t : T}> 
@@ -62,16 +79,19 @@ Inductive valid_references (m : mem) : tm -> Prop :=
 
 Local Ltac _vr tt :=
   match goal with
-  (* irrelevant for unit, nat, and var *)
-  | H : valid_references _ <{fn _ _ _ }> |- _ => tt H
-  | H : valid_references _ <{call _ _ }> |- _ => tt H
-  | H : valid_references _ <{& _ : _  }> |- _ => tt H
-  | H : valid_references _ <{new _ : _}> |- _ => tt H
-  | H : valid_references _ <{* _      }> |- _ => tt H
-  | H : valid_references _ <{_ := _   }> |- _ => tt H
-  | H : valid_references _ <{acq _ _  }> |- _ => tt H
-  | H : valid_references _ <{cr _ _   }> |- _ => tt H
-  | H : valid_references _ <{spawn _  }> |- _ => tt H
+  | H : valid_references _ <{unit        }> |- _ => clear H
+  | H : valid_references _ <{nat _       }> |- _ => clear H
+  | H : valid_references _ <{var _       }> |- _ => clear H
+  | H : valid_references _ <{fn _ _ _    }> |- _ => tt H
+  | H : valid_references _ <{call _ _    }> |- _ => tt H
+  | H : valid_references _ <{& _ : _     }> |- _ => tt H
+  | H : valid_references _ <{new _ : _   }> |- _ => tt H
+  | H : valid_references _ <{init _ _ : _}> |- _ => tt H
+  | H : valid_references _ <{* _         }> |- _ => tt H
+  | H : valid_references _ <{_ := _      }> |- _ => tt H
+  | H : valid_references _ <{acq _ _     }> |- _ => tt H
+  | H : valid_references _ <{cr _ _      }> |- _ => tt H
+  | H : valid_references _ <{spawn _     }> |- _ => tt H
   end.
 
 Ltac inv_vr  := _vr inv.
@@ -81,50 +101,67 @@ Ltac invc_vr := _vr invc.
 (* auxiliary lemmas                                                          *)
 (* ------------------------------------------------------------------------- *)
 
-Lemma vr_tstep_alloc_term : forall m t1 t2 ad t T,
+Lemma vr_tstep_init_term : forall m t1 t2 ad t,
   valid_references m t1 ->
-  t1 --[e_alloc ad t T]--> t2 ->
+  t1 --[e_init ad t]--> t2 ->
   valid_references m t.
 Proof.
-  intros. ind_tstep; inv_vr; eauto using valid_references.
+  intros. ind_tstep; invc_vr; eauto.
 Qed.
 
-Local Lemma vr_tstep_write_term : forall m t1 t2 ad t T,
+Lemma vr_tstep_write_term : forall m t1 t2 ad t,
   valid_references m t1 ->
-  t1 --[e_write ad t T]--> t2 ->
+  t1 --[e_write ad t]--> t2 ->
   valid_references m t.
 Proof.
-  intros. ind_tstep; inv_vr; eauto.
+  intros. ind_tstep; invc_vr; eauto.
 Qed.
 
-Lemma vr_tstep_write_addr : forall m t1 t2 ad t T,
+Lemma vr_tstep_write_addr : forall m t1 t2 ad t,
   valid_references m t1 ->
-  t1 --[e_write ad t T]--> t2 ->
+  t1 --[e_write ad t]--> t2 ->
   ad < #m.
 Proof.
   intros. ind_tstep; repeat invc_vr; eauto.
 Qed.
 
-Lemma valid_write_effect1 : forall t1 t2 ad t T,
+Lemma valid_init_effect : forall m t1 t2 ad t,
   well_typed_term t1 ->
-  (* --- *)
-  t1 --[e_write ad t T]--> t2 ->
-  exists Te, empty |-- t is Te /\ T = `w&Te`.
-Proof.
-  intros * [T' ?] **. generalize dependent T'.
-  ind_tstep; intros; invc_typeof; eauto.
-  invc_typeof. eauto.
-Qed.
-
-Lemma valid_write_effect2 : forall m t1 t2 ad t T,
   valid_references m t1 ->
   (* --- *)
-  t1 --[e_write ad t `w&T`]--> t2 ->
-  m[ad].T = `w&T`.
+  t1 --[e_init ad t]--> t2 ->
+  (exists T, empty |-- t is `Safe T` /\ m[ad].T = `r&T`) \/
+  (exists T, empty |-- t is T        /\ m[ad].T = `x&T`) \/
+  (exists T, empty |-- t is T        /\ m[ad].T = `w&T`).
+Proof.
+  intros * [T ?] **. gendep T.
+  ind_tstep; intros; repeat invc_typeof; repeat invc_vr; eauto.
+Qed.
+
+Lemma valid_write_effect : forall m t1 t2 ad t,
+  well_typed_term t1 ->
+  valid_references m t1 ->
+  (* --- *)
+  t1 --[e_write ad t]--> t2 ->
+  (exists T, empty |-- t is T /\ m[ad].T = `w&T`).
+Proof.
+  intros * [T ?] **. gendep T.
+  ind_tstep; intros; repeat invc_typeof; repeat invc_vr; eauto.
+Qed.
+
+Corollary valid_write_type : forall m t1 t2 ad t T,
+  well_typed_term t1 ->
+  valid_references m t1 ->
+  (* --- *)
+  t1 --[e_write ad t]--> t2 ->
+  empty |-- t is T <-> m[ad].T = `w&T`.
 Proof.
   intros.
-  ind_tstep; intros; invc_vr; eauto.
-  invc_vr. eauto.
+  assert (exists T, empty |-- t is T /\ m[ad].T = `w&T`) as [Te [? ?]]
+      by eauto using valid_write_effect.
+  split; intros.
+  - apply_deterministic_typing. assumption.
+  - invc_eq. assumption.
 Qed.
 
 (* ------------------------------------------------------------------------- *)
@@ -137,48 +174,65 @@ Lemma vr_subst : forall m t tx x,
   valid_references m <{[x := tx] t}>.
 Proof.
   intros.
-  induction t; try inv_vr; eauto using valid_references;
+  induction t; repeat invc_vr; eauto using valid_references;
   simpl; destruct str_eq_dec; eauto using valid_references.
 Qed.
 
-Lemma vr_mem_add : forall m t tT,
+Lemma vr_mem_add : forall m t c,
   valid_references m t ->
-  valid_references (m +++ tT) t.
+  valid_references (m +++ c) t.
 Proof.
   intros. induction t; try invc_vr; eauto using valid_references;
-  (eapply vr_refR || eapply vr_refX || eapply vr_refW || eapply vr_cr);
+  try (constructor; sigma; eauto);
+  (eapply vr_refR || eapply vr_refX || eapply vr_refW); sigma; eauto.
+Qed.
+
+Local Ltac solve_mem_set :=
+  intros ? t **; induction t; invc_vr; eauto using valid_references;
+  try match goal with H1 : _[?ad1].T = _, H2 : _[?ad2].T = _ |- _ =>
+    destruct (nat_eq_dec ad1 ad2); subst; try invc_eq
+  end;
+  (constructor || eapply vr_refR || eapply vr_refX || eapply vr_refW);
   sigma; eauto.
-Qed.
 
-Local Ltac invc_eq := 
-  match goal with H1 : ?x = ?a, H2 : ?x = ?b |- _ =>
-    rewrite H1 in H2; invc H2
-  end.
-
-Lemma vr_mem_setW : forall m t ad te T Te,
-  ad < #m ->
-  T = `w&Te` ->
-  m[ad].T = `w&Te` ->
-  empty |-- te is Te ->
+Lemma vr_mem_setR : forall m t te ad T,
+  m[ad].T = `r&T` ->
+  empty |-- te is `Safe T` ->
   (* --- *)
   valid_references m t ->
-  valid_references m[ad.tT <- te T] t.
-Proof.
-  intros. subst. induction t; try invc_vr; eauto using valid_references;
-  (eapply vr_refR || eapply vr_refX || eapply vr_refW || eapply vr_cr);
-  sigma; eauto; omicron; trivial; invc_eq; trivial.
-Qed.
+  valid_references m[ad.t <- te] t.
+Proof. solve_mem_set. Qed.
 
-Lemma vr_mem_setX : forall m t ad X,
-  ad < #m ->
+Lemma vr_mem_setX : forall m t te ad T,
+  m[ad].T = `x&T` ->
+  empty |-- te is T ->
   (* --- *)
   valid_references m t ->
-  valid_references m[ad.X <- X] t.
-Proof.
-  intros. induction t; try invc_vr; eauto using valid_references;
-  (eapply vr_refR || eapply vr_refX || eapply vr_refW || eapply vr_cr);
+  valid_references m[ad.t <- te] t.
+Proof. solve_mem_set. Qed.
+
+Lemma vr_mem_setW : forall m t te ad T,
+  m[ad].T = `w&T` ->
+  empty |-- te is T ->
+  (* --- *)
+  valid_references m t ->
+  valid_references m[ad.t <- te] t.
+Proof. solve_mem_set. Qed.
+
+Local Ltac solve_mem_acq_rel :=
+  intros ? t **; induction t; try invc_vr; eauto using valid_references;
+  (constructor || eapply vr_refR || eapply vr_refX || eapply vr_refW);
   sigma; eauto; omicron; eauto.
-Qed.
+
+Lemma vr_mem_acq : forall m t ad,
+  valid_references m t ->
+  valid_references m[ad.X <- true] t.
+Proof. solve_mem_acq_rel. Qed.
+
+Lemma vr_mem_rel : forall m t ad,
+  valid_references m t ->
+  valid_references m[ad.X <- false] t.
+Proof. solve_mem_acq_rel. Qed.
 
 (* none -------------------------------------------------------------------- *)
 
@@ -194,107 +248,162 @@ Qed.
 
 (* alloc ------------------------------------------------------------------- *)
 
-Lemma vr_preservation_mem_alloc : forall m t1 t2 t T X,
+Lemma vr_preservation_mem_alloc : forall m t1 t2 T X,
   well_typed_term t1 ->
   valid_references m t1 ->
   (* --- *)
   forall_memory m (valid_references m) ->
-  t1 --[e_alloc (#m) t T]--> t2 ->
-  forall_memory (m +++ (t, T, X)) (valid_references (m +++ (t, T, X))).
+  t1 --[e_alloc (#m) T]--> t2 ->
+  forall_memory (m +++ (None, T, X)) (valid_references (m +++ (None, T, X))).
 Proof.
-  intros ** ad. omicron;
-  eauto using vr_mem_add, valid_references; (* optimization *)
-  eauto using vr_mem_add, vr_tstep_alloc_term.
+  intros ** ? ? ?. omicron; eauto using vr_mem_add; discriminate.
 Qed.
 
-Lemma vr_preservation_alloc : forall m t1 t2 t T X,
+Lemma vr_preservation_alloc : forall m t1 t2 T X,
   well_typed_term t1 ->
   (* --- *)
   valid_references m t1 ->
-  t1 --[e_alloc (#m) t T]--> t2 ->
-  valid_references (m +++ (t, T, X)) t2.
+  t1 --[e_alloc (#m) T]--> t2 ->
+  valid_references (m +++ (None, T, X)) t2.
 Proof.
-  intros * [T ?] **. generalize dependent T.
-  ind_tstep; intros; inv_vr; inv_typeof;
-  eauto using vr_mem_add, valid_references;
-  (eapply vr_refR || eapply vr_refX || eapply vr_refW || eapply vr_cr);
-  sigma; eauto using type_of, empty_eq_safe_empty.
+  intros * [T ?] **. gendep T.
+  ind_tstep; intros; invc_typeof; invc_vr;
+  constructor; sigma; eauto using vr_mem_add.
 Qed.
 
-Lemma vr_preservation_unt_alloc : forall m t1 t2 tu ad t T X,
+Lemma vr_preservation_unt_alloc : forall m t1 t2 tu ad T X,
   valid_references m tu ->
-  t1 --[e_alloc ad t T]--> t2 ->
-  valid_references (m +++ (t, T, X)) tu.
+  t1 --[e_alloc ad T]--> t2 ->
+  valid_references (m +++ (None, T, X)) tu.
+Proof.
+  intros. ind_tstep; eauto using vr_mem_add.
+Qed.
+
+(* init -------------------------------------------------------------------- *)
+
+Lemma vr_preservation_mem_init : forall m t1 t2 ad t,
+  well_typed_term t1 ->
+  valid_references m t1 ->
+  (* --- *)
+  forall_memory m (valid_references m) ->
+  t1 --[e_init ad t]--> t2 ->
+  forall_memory m[ad.t <- t] (valid_references m[ad.t <- t]).
+Proof.
+  intros ** ? ? Had.
+  assert (
+    (exists T, empty |-- t is `Safe T` /\ m[ad].T = `r&T`) \/
+    (exists T, empty |-- t is T        /\ m[ad].T = `x&T`) \/
+    (exists T, empty |-- t is T        /\ m[ad].T = `w&T`)
+  ) as [[? [? ?]] | [[? [? ?]] | [? [? ?]]]]
+    by eauto using valid_init_effect;
+  repeat omicron; try discriminate; invc Had;
+  eauto using vr_mem_setR, vr_mem_setX, vr_mem_setW, vr_tstep_init_term.
+Qed.
+
+Lemma vr_preservation_init : forall m t1 t2 ad t,
+  well_typed_term t1 ->
+  (* --- *)
+  ad < #m ->
+  valid_references m t1 ->
+  t1 --[e_init ad t]--> t2 ->
+  valid_references (m[ad.t <- t]) t2.
 Proof.
   intros.
-  ind_tstep; eauto using vr_mem_add, valid_references.
+  assert (
+    (exists T, empty |-- t is `Safe T` /\ m[ad].T = `r&T`) \/
+    (exists T, empty |-- t is T        /\ m[ad].T = `x&T`) \/
+    (exists T, empty |-- t is T        /\ m[ad].T = `w&T`)
+  ) as [[? [? ?]] | [[? [? ?]] | [? [? ?]]]]
+    by eauto using valid_init_effect;
+  ind_tstep; invc_wtt; invc_vr;
+  eauto using vr_mem_setR, vr_mem_setX, vr_mem_setW, valid_references;
+  try solve [constructor; sigma; eauto; omicron; eauto];
+  invc_eq; (eapply vr_refR || eapply vr_refX || eapply vr_refW); sigma; eauto.
+Qed.
+
+Lemma vr_preservation_unt_init : forall m t1 t2 tu ad t,
+  well_typed_term t1 ->
+  valid_references m t1 ->
+  (* --- *)
+  ad < #m ->
+  valid_references m tu ->
+  t1 --[e_init ad t]--> t2 ->
+  valid_references m[ad.t <- t] tu.
+Proof.
+  intros.
+  assert (
+    (exists T, empty |-- t is `Safe T` /\ m[ad].T = `r&T`) \/
+    (exists T, empty |-- t is T        /\ m[ad].T = `x&T`) \/
+    (exists T, empty |-- t is T        /\ m[ad].T = `w&T`)
+  ) as [[? [? ?]] | [[? [? ?]] | [? [? ?]]]]
+    by eauto using valid_init_effect;
+  eauto using vr_mem_setR, vr_mem_setX, vr_mem_setW.
 Qed.
 
 (* read -------------------------------------------------------------------- *)
 
-Lemma vr_preservation_read : forall m t1 t2 ad,
-  valid_references m m[ad].t ->
+Lemma vr_preservation_read : forall m t1 t2 ad t,
+  m[ad].t = Some t ->
+  valid_references m t ->
   (* --- *)
   valid_references m t1 ->
-  t1 --[e_read ad m[ad].t]--> t2 ->
+  t1 --[e_read ad t]--> t2 ->
   valid_references m t2.
 Proof.
-  intros.
-  ind_tstep; inv_vr; eauto using valid_references.
+  intros. ind_tstep; invc_vr; eauto using valid_references.
 Qed.
 
 (* write ------------------------------------------------------------------- *)
 
-Lemma vr_preservation_mem_write : forall m t1 t2 ad t T,
+Lemma vr_preservation_mem_write : forall m t1 t2 ad t,
   well_typed_term t1 ->
   valid_references m t1 ->
   (* --- *)
   ad < #m ->
   forall_memory m (valid_references m) ->
-  t1 --[e_write ad t T]--> t2 ->
-  forall_memory m[ad.tT <- t T] (valid_references m[ad.tT <- t T]).
+  t1 --[e_write ad t]--> t2 ->
+  forall_memory m[ad.t <- t] (valid_references m[ad.t <- t]).
 Proof.
-  intros ** ?.
-  assert (exists Te, empty |-- t is Te /\ T = `w&Te`) as [Te [? ?]]
-    by eauto using valid_write_effect1.
-  omicron; eauto using vr_mem_setW, valid_write_effect2, vr_tstep_write_term.
+  intros ** ? ? Had.
+  assert (exists T, empty |-- t is T /\ m[ad].T = `w&T`) as [Te [? ?]]
+    by eauto using valid_write_effect.
+  omicron; invc Had; eauto using vr_mem_setW, vr_tstep_write_term.
 Qed.
 
-Lemma vr_preservation_write : forall m t1 t2 ad t T,
+Lemma vr_preservation_write : forall m t1 t2 ad t,
   well_typed_term t1 ->
   (* --- *)
   ad < #m ->
   valid_references m t1 ->
-  t1 --[e_write ad t T]--> t2 ->
-  valid_references (m[ad.tT <- t T]) t2.
+  t1 --[e_write ad t]--> t2 ->
+  valid_references (m[ad.t <- t]) t2.
 Proof.
   intros.
-  assert (exists Te, empty |-- t is Te /\ T = `w&Te`) as [Te [? ?]]
-    by eauto using valid_write_effect1.
+  assert (exists T, empty |-- t is T /\ m[ad].T = `w&T`) as [Te [? ?]]
+    by eauto using valid_write_effect.
   ind_tstep; invc_wtt; invc_vr;
-  eauto using vr_mem_setW, valid_write_effect2, valid_references.
-  eapply vr_cr; sigma; eauto.
+  eauto using vr_mem_setW, valid_references;
+  constructor; sigma; eauto; omicron; eauto.
 Qed.
 
-Lemma vr_preservation_unt_write : forall m t1 t2 tu ad t T,
+Lemma vr_preservation_unt_write : forall m t1 t2 tu ad t,
   well_typed_term t1 ->
   valid_references m t1 ->
   (* --- *)
   ad < #m ->
   valid_references m tu ->
-  t1 --[e_write ad t T]--> t2 ->
-  valid_references m[ad.tT <- t T] tu.
+  t1 --[e_write ad t]--> t2 ->
+  valid_references m[ad.t <- t] tu.
 Proof.
   intros.
-  assert (exists Te, empty |-- t is Te /\ T = `w&Te`) as [Te [? ?]]
-    by eauto using valid_write_effect1.
-  subst.
-  eauto using vr_mem_setW, valid_write_effect2.
+  assert (exists T, empty |-- t is T /\ m[ad].T = `w&T`) as [Te [? ?]]
+    by eauto using valid_write_effect.
+  eauto using vr_mem_setW.
 Qed.
 
 (* acq --------------------------------------------------------------------- *)
 
-Lemma vr_preservation_mem_acq : forall m t1 t2 ad t X,
+Lemma vr_preservation_mem_acq : forall m t1 t2 ad t,
   forall_memory m well_typed_term ->
   well_typed_term t1 ->
   valid_references m t1 ->
@@ -302,37 +411,37 @@ Lemma vr_preservation_mem_acq : forall m t1 t2 ad t X,
   ad < #m ->
   forall_memory m (valid_references m) ->
   t1 --[e_acq ad t]--> t2 ->
-  forall_memory m[ad.X <- X] (valid_references m[ad.X <- X]).
+  forall_memory m[ad.X <- true] (valid_references m[ad.X <- true]).
 Proof.
-  intros ** ?. omicron; eauto using vr_mem_setX.
+  intros ** ? ? ?. omicron; eauto using vr_mem_acq.
 Qed.
 
-Lemma vr_preservation_acq : forall m t1 t2 ad X,
-  forall_memory m (valid_references m) ->
+Lemma vr_preservation_acq : forall m t1 t2 ad t,
+  m[ad].t = Some t ->
+  valid_references m t ->
   (* --- *)
   ad < #m ->
   valid_references m t1 ->
-  t1 --[e_acq ad m[ad].t]--> t2 ->
-  valid_references m[ad.X <- X] t2.
+  t1 --[e_acq ad t]--> t2 ->
+  valid_references m[ad.X <- true] t2.
 Proof.
-  intros.
-  ind_tstep; invc_vr; eauto using vr_mem_setX, valid_references.
-  repeat invc_vr; eauto using vr_subst, vr_mem_setX, valid_references.
-  eapply vr_cr; sigma; eauto.
+  intros. ind_tstep; repeat invc_vr;
+  eauto using vr_mem_acq, vr_subst, valid_references;
+  constructor; sigma; eauto; omicron; eauto.
 Qed.
 
-Lemma vr_preservation_unt_acq : forall m t1 t2 tu ad t X,
+Lemma vr_preservation_unt_acq : forall m t1 t2 tu ad t,
   ad < #m ->
   valid_references m tu ->
   t1 --[e_acq ad t]--> t2 ->
-  valid_references m[ad.X <- X] tu.
+  valid_references m[ad.X <- true] tu.
 Proof.
-  eauto using vr_mem_setX.
+  eauto using vr_mem_acq.
 Qed.
 
 (* rel --------------------------------------------------------------------- *)
 
-Lemma vr_preservation_mem_rel : forall m t1 t2 ad X,
+Lemma vr_preservation_mem_rel : forall m t1 t2 ad,
   forall_memory m well_typed_term ->
   well_typed_term t1 ->
   valid_references m t1 ->
@@ -340,29 +449,28 @@ Lemma vr_preservation_mem_rel : forall m t1 t2 ad X,
   ad < #m ->
   forall_memory m (valid_references m) ->
   t1 --[e_rel ad]--> t2 ->
-  forall_memory m[ad.X <- X] (valid_references m[ad.X <- X]).
+  forall_memory m[ad.X <- false] (valid_references m[ad.X <- false]).
 Proof.
-  intros ** ?. omicron; eauto using vr_mem_setX.
+  intros ** ? ? ?. omicron; eauto using vr_mem_rel.
 Qed.
 
-Lemma vr_preservation_rel : forall m t1 t2 ad X,
+Lemma vr_preservation_rel : forall m t1 t2 ad,
   ad < #m ->
   valid_references m t1 ->
   t1 --[e_rel ad]--> t2 ->
-  valid_references m[ad.X <- X] t2.
+  valid_references m[ad.X <- false] t2.
 Proof.
-  intros.
-  ind_tstep; invc_vr; eauto using vr_mem_setX, valid_references.
-  eapply vr_cr; sigma; eauto.
+  intros. ind_tstep; invc_vr; eauto using vr_mem_rel, valid_references;
+  constructor; sigma; eauto; omicron; eauto.
 Qed.
 
-Lemma vr_preservation_unt_rel : forall m t1 t2 tu ad X,
+Lemma vr_preservation_unt_rel : forall m t1 t2 tu ad,
   ad < #m ->
   valid_references m tu ->
   t1 --[e_rel ad]--> t2 ->
-  valid_references m[ad.X <- X] tu.
+  valid_references m[ad.X <- false] tu.
 Proof.
-  eauto using vr_mem_setX.
+  eauto using vr_mem_rel.
 Qed.
 
 (* spawn ------------------------------------------------------------------- *)
@@ -385,6 +493,12 @@ Qed.
 
 (* ------------------------------------------------------------------------- *)
 
+Ltac destruct_forall := 
+  match goal with
+  | |- forall_threads _[_ <- _] _          => intros tid'; omicron
+  | |- forall_threads (_[_ <- _] +++ _) _  => intros tid'; omicron
+  end.
+
 Theorem vr_preservation : forall m1 m2 ths1 ths2 tid e,
   forall_program m1 ths1 well_typed_term ->
   (* --- *)
@@ -392,11 +506,15 @@ Theorem vr_preservation : forall m1 m2 ths1 ths2 tid e,
   m1 / ths1 ~~[tid, e]~~> m2 / ths2 ->
   forall_program m2 ths2 (valid_references m2).
 Proof.
-  split_preservation.
+  intros * [? ?] [? ?] ?.
+  invc_cstep; try invc_mstep; split; try destruct_forall; trivial.
   - eauto using vr_preservation_none.
   - eauto using vr_preservation_mem_alloc.
   - eauto using vr_preservation_alloc.
   - eauto using vr_preservation_unt_alloc.
+  - eauto using vr_preservation_mem_init.
+  - eauto using vr_preservation_init.
+  - eauto using vr_preservation_unt_init.
   - eauto using vr_preservation_read.
   - eauto using vr_preservation_mem_write.
   - eauto using vr_preservation_write.
@@ -410,22 +528,5 @@ Proof.
   - eauto using vr_preservation_spawn.
   - eauto using vr_preservation_spawned.
   - eauto using valid_references.
-Qed.
-
-(* ------------------------------------------------------------------------- *)
-
-Corollary vr_cstep_preservation : forall m1 m2 ths1 ths2 tid e,
-  forall_memory  m1   well_typed_term ->
-  forall_threads ths1 well_typed_term ->
-  (* --- *)
-  forall_memory m1 (valid_references m1) ->
-  forall_threads ths1 (valid_references m1) ->
-  m1 / ths1 ~~[tid, e]~~> m2 / ths2 ->
-  forall_threads ths2 (valid_references m2).
-Proof.
-  intros.
-  assert (forall_program m2 ths2 (valid_references m2))
-    by (eapply vr_preservation; eauto).
-  destruct_forall_program. assumption.
 Qed.
 
