WellTypedTerm.v
@@ -42,6 +42,11 @@ Local Lemma inv_wtt_new : forall t T,
   well_typed_term t.
 Proof. solve_wtt_inversion. Qed.
 
+Local Lemma inv_wtt_init : forall ad t T,
+  well_typed_term <{init ad t : T}> ->
+  well_typed_term t.
+Proof. solve_wtt_inversion. Qed.
+
 Local Lemma inv_wtt_load : forall t,
   well_typed_term <{*t}> ->
   well_typed_term t.
@@ -67,38 +72,33 @@ Local Lemma inv_wtt_spawn : forall t,
   well_typed_term t.
 Proof. solve_wtt_inversion. Qed.
 
-Local Notation wtt := (well_typed_term ).
+Local Notation wtt := (well_typed_term).
 
 Ltac invc_wtt :=
   match goal with
-  (* irrelevant for unit and nat *)
-  | H : wtt <{var _    }> |- _ => eapply inv_wtt_var   in H; contradiction
-  | H : wtt <{fn _ _ _ }> |- _ => eapply inv_wtt_fun   in H as [? ?]
-  | H : wtt <{call _ _ }> |- _ => eapply inv_wtt_call  in H as [? ?]
-  | H : wtt <{& _ : _  }> |- _ => eapply inv_wtt_ref   in H as [[? ?] | [? ?]]
-  | H : wtt <{new _ : _}> |- _ => eapply inv_wtt_new   in H
-  | H : wtt <{* _      }> |- _ => eapply inv_wtt_load  in H
-  | H : wtt <{_ := _   }> |- _ => eapply inv_wtt_asg   in H as [? ?]
-  | H : wtt <{acq _ _  }> |- _ => eapply inv_wtt_acq   in H as [? ?]
-  | H : wtt <{cr _ _   }> |- _ => eapply inv_wtt_cr    in H
-  | H : wtt <{spawn _  }> |- _ => eapply inv_wtt_spawn in H
+  | H : wtt <{unit        }> |- _ => clear H
+  | H : wtt <{nat _       }> |- _ => clear H
+  | H : wtt <{var _       }> |- _ => eapply inv_wtt_var   in H; contradiction
+  | H : wtt <{fn _ _ _    }> |- _ => eapply inv_wtt_fun   in H as [? ?]
+  | H : wtt <{call _ _    }> |- _ => eapply inv_wtt_call  in H as [? ?]
+  | H : wtt <{& _ : _     }> |- _ => eapply inv_wtt_ref   in H
+                                                    as [[? ?] | [[? ?] | [? ?]]]
+  | H : wtt <{new _ : _   }> |- _ => eapply inv_wtt_new   in H
+  | H : wtt <{init _ _ : _}> |- _ => eapply inv_wtt_init  in H
+  | H : wtt <{* _         }> |- _ => eapply inv_wtt_load  in H
+  | H : wtt <{_ := _      }> |- _ => eapply inv_wtt_asg   in H as [? ?]
+  | H : wtt <{acq _ _     }> |- _ => eapply inv_wtt_acq   in H as [? ?]
+  | H : wtt <{cr _ _      }> |- _ => eapply inv_wtt_cr    in H
+  | H : wtt <{spawn _     }> |- _ => eapply inv_wtt_spawn in H
   end.
 
 (* ------------------------------------------------------------------------- *)
 (* auxiliary lemmas                                                          *)
 (* ------------------------------------------------------------------------- *)
 
-Lemma wtt_tstep_alloc_term : forall t1 t2 ad t T,
+Lemma wtt_tstep_write_term : forall t1 t2 ad t,
   well_typed_term t1 ->
-  t1 --[e_alloc ad t T ]--> t2 ->
-  well_typed_term t.
-Proof.
-  intros. ind_tstep; invc_wtt; eauto.
-Qed.
-
-Lemma wtt_tstep_write_term : forall t1 t2 ad t T,
-  well_typed_term t1 ->
-  t1 --[e_write ad t T ]--> t2 ->
+  t1 --[e_write ad t]--> t2 ->
   well_typed_term t.
 Proof.
   intros. ind_tstep; invc_wtt; eauto.
